vminus/Compiler.v
@@ -1,3 +1,4 @@
+(* * Compiler: An Imp to Vminus Compiler *)
 (* -------------------------------------------------------------------------- *
  *                     Vellvm - the Verified LLVM project                     *
  *                                                                            *
@@ -8,9 +9,6 @@
  *   3 of the License, or (at your option) any later version.                 *
  ---------------------------------------------------------------------------- *)
 
-
-(* ################################################################# *)
-(** * Imp to Vminus Compiler *)
 
 (** Imports, instantiated with the list implementation of 
     control-flow graphs. *)
@@ -23,123 +21,283 @@ Require Import Vminus.CFG.
 Require Import Vminus.ListCFG.
 Import ListCFG.
 
+
 (* ################################################################# *)
-(** * Compiling Expressions *)
+(** * Imp to Vminus Compiler *)
 
-(** Compilation context for expressions.  The state monad keeps track
-    of the list of generated uids so that we can generate fresh names. *)
+(** This file implements a compiler from a (slight variant of) the Software
+Foundations Imp language (see [Imp.v]) to Vminus.  Importantly, this variant of
+Imp and the Vminus language share the same notion of global, mutable memory
+states, so the compilation of Imp identifiers into Vminus addresses is trivial.
+*)
 
-Notation ectmon := (ST (list uid)).
+(** The compiler and its correctness proof demonstrate the use of
+_monotonic state_---essentially the idea that the compiler only "extends" the
+state, either by generating new fresh identifiers.
 
-(** Generate a fresh uid. *)
+For the sake of simplicity, this compiler doesn't perform any optimizations.  It
+uses a straightforward strategy of translating each Imp assignment command to a
+separate Vminus block, which makes stating the correctness invariants easier, at
+the expense of generating poor straight-line code.
 
-Definition fresh : ectmon uid :=
-  fun is =>
-  let i := Uid.fresh is in
-  (i::is, i).
+The compiler will also serve as a vehicle for exploring QuickChick testing.
 
-Definition strun {A:Set} (m:ectmon A) (l:list uid) : A :=
+*)
+
+(**  ------------------------------------------------------------------------- *)
+(** *** An example of translating Imp to Vminus:
+
+An Imp program:
+
+[IFZ Z THEN X ::= 1;; Y ::= 2 ELSE SKIP]
+
+And one possible translation to Vminus:
+
+
+l0:
+  %z = load Z
+  cbr %z l1 l3
+
+l1:           // block for X ::= 1
+  store X 1
+  br l2
+
+l2:           // block for Y ::= 2
+  store Y 2
+  br l3
+
+l3:
+  ret
+
+
+*)
+
+
+(**  ------------------------------------------------------------------------- *)
+(* ################################################################# *)
+(** * The Compilation Monad *)
+
+(** One issue in building a compiler that targets an SSA language like
+Vminus is generating the identifiers used for labels and local variables.  A key
+part of the correctness proof will be establishing the freshness and uniqueness
+properties of these identifiers.
+ *)
+(** The [FRESH] monad provides a compilation context for expressions and commands.
+    [FRESH] is just a state monad in which the state keeps track of the list of
+    generated uids so that we can generate fresh names.  *)
+
+Notation FRESH := (ST (list uid)).
+
+(** A monad operation that generates a unique identifer [uid]. Note that the the
+[Atom] library guarantees that [uid] is distinct from any element of [ids]. *)
+
+Definition fresh : FRESH uid :=
+  fun ids =>
+  let uid := Uid.fresh ids in
+  (uid::ids, uid).
+
+(** We can _run_ the monad computation starting from any initial list of uids
+that should be avoided. *)
+
+Definition strun {A:Set} (m:FRESH A) (l:list uid) : A :=
   snd (m l).
 
-(* ================================================================= *)
-(** ** Compiling binops. *)
+(**  ------------------------------------------------------------------------- *)
+(* ################################################################# *)
+(** * Compiling binops. *)
 
-(** Compile a general binary operation. *)
+(** The result of compiling an expression is a Vminus value that stores the
+result, plus a sequence of intructions (if any) needed to compute that value.  *)
 
-(*! Section comp_bop *)
+(** We can factor all of the shared code for compiling binary operations into a
+monadic combinator. It first compiles the left expression, then the right
+expression. Then it generates a fresh local identifier that will hold the
+computed result.  The instruction sequence concatenates the code for the two
+subexpressions and appends the instruction that performs the binary
+operation. *)
 
-Definition comp_bop (b:bop) (e1 e2: ectmon (val * list insn)) : ectmon (val * list insn) :=
+
+Definition comp_bop (b:bop) (e1 e2: FRESH (val * list insn)) : FRESH (val * list insn) :=
   '(v1, c1) <- e1;
   '(v2, c2) <- e2;
   'r <- fresh; 
   mret (val_uid r, (c1 ++ c2 ++ [(r, cmd_bop b v1 v2)])).
 
-(** Compile an arithmetic expression. *)
+(**  ------------------------------------------------------------------------- *)
+(* ################################################################# *)
+(** * Compiling arithmetic expressions. *)
 
-(*! Section comp_aexp *)
+(** The translation of an Imp [aexp] is mostly handled by [comp_bop].
 
-Fixpoint comp_aexp (a:aexp) : ectmon (val * list insn) :=
+The only interesting case is that for compiling Imp identifiers.  However, since
+the Imp global state and Vminus global state are the same, we simply translate
+a reference to an Imp identifier into a load from that identifier, treated as an
+address.
+*)
+
+
+Fixpoint comp_aexp (a:aexp) : FRESH (val * list insn) :=
   match a with
     | ANum n => mret (val_nat n, [])
     | AId i => 'r <- fresh; mret (val_uid r, [(r, cmd_load i)])
-    | APlus a1 a2 => (*!*)comp_bop bop_add (comp_aexp a1) (comp_aexp a2)
-                    (*! comp_bop bop_add (comp_aexp a1) (comp_aexp a1) *)
-    | AMinus a1 a2 => (*! *) comp_bop bop_sub (comp_aexp a1) (comp_aexp a2)
-                     (*! comp_bop bop_sub (comp_aexp a1) (comp_aexp a1) *)
-    | AMult a1 a2 => (*! *) comp_bop bop_mul (comp_aexp a1) (comp_aexp a2)
-                    (*! comp_bop bop_mul (comp_aexp a1) (comp_aexp a1) *)
+    | APlus a1 a2 => comp_bop bop_add (comp_aexp a1) (comp_aexp a2)
+    | AMinus a1 a2 => comp_bop bop_sub (comp_aexp a1) (comp_aexp a2)
+    | AMult a1 a2 => comp_bop bop_mul (comp_aexp a1) (comp_aexp a2)
   end.
 
-(* ================================================================= *)
-(** ** Compiling boolean expressions. *)
+(**  ------------------------------------------------------------------------- *)
+(* ################################################################# *)
+(** * Compiling boolean expressions. *)
 
-(*! Section comp_bexp *)
-Fixpoint comp_bexp (b:bexp) : ectmon (val * list insn) :=
+
+(** Vminus doesn't have booleans, it has only natural numbers, so we have
+to translate Imp values [BTrue] and [BFalse] to [val_nat 1] and [val_nat 0]
+respectively.
+
+Vminus does not have any unary operations, so logical negation translates into a
+comparison with [0].
+*)
+
+Fixpoint comp_bexp (b:bexp) : FRESH (val * list insn) :=
   match b with
-    | BTrue => (*! *) mret (val_nat 1, []) (*! ret (val_nat 0, []) *)
+    | BTrue => mret (val_nat 1, [])
     | BFalse => mret (val_nat 0, [])
     | BEq a1 a2 => comp_bop bop_eq (comp_aexp a1) (comp_aexp a2)
-    | BLe a1 a2 => (*! *) comp_bop bop_le (comp_aexp a1) (comp_aexp a2)
-                  (*! comp_bop bop_le (comp_aexp a1) (comp_aexp a1) *)
-    | BAnd b1 b2 => (*!*) comp_bop bop_and (comp_bexp b1) (comp_bexp b2)
-                   (*! comp_bop bop_and (comp_bexp b1) (comp_bexp b1) *)
-    | BNot b1 => (*!*) comp_bop bop_eq (comp_bexp b1) (mret (val_nat 0, []))
-                (*! comp_bop bop_eq (comp_bexp b1) (ret (val_nat 1, [])) *)
+    | BLe a1 a2 => comp_bop bop_le (comp_aexp a1) (comp_aexp a2)
+    | BAnd b1 b2 => comp_bop bop_and (comp_bexp b1) (comp_bexp b2)
+    | BNot b1 => comp_bop bop_eq (comp_bexp b1) (mret (val_nat 0, []))
   end.
 
+(**  ------------------------------------------------------------------------- *)
+(* ################################################################# *)
+(** * Command compilation strategy *)
 
+(** To compile Imp commands to Vminus, observe that a single Imp command
+such as [IFZ] or [WHILE] will translate into a collection of Vminus basic
+blocks.  Therefore the command compiler will need to produce that list of
+blocks, as well as have the infrastructure provide a mechanism for indicating
+how the blocks should be connected to form a control-flow graph.
 
-Definition comp_store (a:aexp) (v:addr) (lr:lbl) : ectmon (list insn) :=
+For this compiler, we've chosen to follow the invariant that when translating an
+Imp command [c], the compiler receives the label of the _continuation block_ to
+which control should pass after executing the code corresponding to [c].  The
+_output_ of the command compiler is a label that designates the entry block of
+the command.  These choices inform the structure of the compiler, which
+traverses the Imp program from right-to-left, threading the control as required.
+
+Another consequence of this decision is that the easiest way to compile
+assignment commands is to place each such command into its own basic block.
+This simplifies the compiler invariants (since we don't have to keep track of
+"partially completed" blocks, and (as we will see) makes relating the Imp
+operational semantics to the Vminus semantics of the compiler output.
+
+There are alternatives that could produce "nicer" Vminus code (e.g. by placing
+sequences of assignment commands into the same basic block, or by traversing the
+Imp program left-to-right), but those alternatives would have a significant
+impact on the simulation relation between the source Imp and target Vminus code.
+
+Note: This compilation strategy also does not introduce phi nodes into the
+generated code.  This design is in-line with the usual way of compiling an
+imperative language to a language like Vminus (or LLVM).  Introduction of phi
+nodes is done as a later phase in the compiler, sometimes called "register
+promotion".
+
+*)
+
+(**  ------------------------------------------------------------------------- *)
+(* ################################################################# *)
+(** * Compiling [store] commands and conditional branches *)
+
+(** Before diving into the full compiler, it is useful to create two helper
+functions, each of which is responsible for generating code that corresponds to
+the last half of a basic block.
+*)
+
+(** [comp_store] emits code that computes an arithmetic expression [a] and
+stores the result into the address [v].  The [k] argument is the "continuation
+label" that is jumped to following the [store].  *)
+
+Definition comp_store (a:aexp) (v:addr) (k:lbl) : FRESH (list insn) :=
   'x <- fresh;
   'y <- fresh;
   '(i, is) <- comp_aexp a; 
   mret (is ++ [ (x, cmd_store v i); 
-               (y, cmd_tmn (tmn_jmp lr)) ]).
+               (y, cmd_tmn (tmn_jmp k)) ]).
 
-Definition comp_cond (b:bexp) (l1 l2:lbl) : ectmon (list insn) :=
+
+(** Similarly, [comp_cond] generates the instructions leading up to a
+conditional branch.  It takes two continuation labels, one for each branch.  *)
+
+Definition comp_cond (b:bexp) (l1 l2:lbl) : FRESH (list insn) :=
   '(v, is) <- comp_bexp b;
   'x <- fresh;
   mret (is ++ [ (x, cmd_tmn (tmn_cbr v l1 l2)) ] ).
 
-(* ================================================================= *)
-(* ** Compiling Commands *)
+(**  ------------------------------------------------------------------------- *)
+(* ################################################################# *)
+(** * Compiling Imp Commands *)
 
-(** State:
-    - list of used block labels
-    - list of used uids
-    - current cfg *)
+(** Just as we needed to thread the list of generated identifiers through the
+expression compiler, we also need to maintain some state when compiling
+commands.
+  
+  - list of used block labels
+
+  - list of used uids
+
+  - list of blocks making up the "current" control-flow graph, to which new
+    blocks will be added
+
+ *)
+
+(** We define another monad, called [CMD] that, in addition to letting us
+generate fresh local identifiers, also keeps track of block labels and generated
+blocks.  *)
 
 Definition cstate := (list lbl * list uid * list block)%type.
-Notation ctmon := (ST cstate).
+Notation CMD := (ST cstate).
 
-Definition fresh_lbl : ctmon lbl :=
+(** Generate a fresh block label *)
+
+Definition fresh_lbl : CMD lbl :=
   fun cs =>
   let '(ls, is, bs) := cs in
   let l := Lbl.fresh ls in 
   (l::ls, is, update bs l [], l).
 
-Definition raise_ectmon {T} (ec:ectmon T) : ctmon T :=
+(** Lift a computation from the [FRESH] monad into the [CMD] monad. *)
+
+Definition liftF {T} (ec:FRESH T) : CMD T :=
   fun cs =>
   let '(ls, is, cfg) := cs in
   let (is', r) := ec is in
   (ls, is', cfg, r).
 
-Definition add_insns (l:lbl) (b:list insn) : ctmon unit :=
+(** Update the instructions at the block with lbl [l] to have the list of instructions [b] *)
+
+Definition add_insns (l:lbl) (b:list insn) : CMD unit :=
   fun cs =>
   let '(ls, is, cfg) := cs in
   (ls, is, update cfg l b, tt).
 
-(** The input [lr] is the label of the block to which
-    control should return after the command is done. 
-    The output is the label of the entry block for the
-    command. *)
+(**  ------------------------------------------------------------------------- *)
+(* ################################################################# *)
+(** * Compiling Imp Commands *)
 
-Fixpoint comp_com (c:Imp.com) (lr:lbl) : ctmon lbl :=
+(** The input [lr] is the "continuation" label of the block to which control
+    should return after the command is done.  The output is the label of the
+    entry block for the command. 
+
+    Note how compiling a sequence [[c1;;c2]] threads the control through the 
+    commands in reverse order.
+*)
+
+Fixpoint comp_com (c:Imp.com) (lr:lbl) : CMD lbl :=
   match c with
     | CSkip => mret lr
     | CAss i a => 
         'l <- fresh_lbl;
-        'b <- raise_ectmon (comp_store a i lr);
+        'b <- liftF (comp_store a i lr);
         '_ <- add_insns l b;
         mret l
     | CSeq c1 c2 =>
@@ -148,25 +306,40 @@ Fixpoint comp_com (c:Imp.com) (lr:lbl) : ctmon lbl :=
         'l1 <- comp_com c1 lr;
         'l2 <- comp_com c2 lr;
         'lh <- fresh_lbl;
-        'b  <- raise_ectmon (comp_cond b l1 l2);
+        'b  <- liftF (comp_cond b l1 l2);
         '_  <- add_insns lh b;
         mret lh
     | CWhile b c => 
         'lh <- fresh_lbl;
         'lb <- comp_com c lh;
-        'b  <- raise_ectmon (comp_cond b lb lr);
+        'b  <- liftF (comp_cond b lb lr);
         '_  <- add_insns lh b;
         mret lh
   end.
 
-Definition comp_prog (c:com) : ctmon (lbl * lbl) :=
+(**  ------------------------------------------------------------------------- *)
+(* ################################################################# *)
+(** * Top-level Compiler *)
+
+(** To turn an Imp command into a full Vminus program, we need to provide the
+command compiler with the label of the "initial continuation", which is just the
+label of a block that immediately halts the program by executing the [tmn_ret]
+instruction.  The result of the program is a pair of labels, [e] for the entry
+point (obtained by compiling the command [c]), and the exit label [r].
+
+*)
+
+Definition comp_prog (c:com) : CMD (lbl * lbl) :=
   'r <- fresh_lbl;
-  'x <- raise_ectmon fresh;
+  'x <- liftF fresh;
   '_ <- add_insns r [(x, cmd_tmn tmn_ret)];
   'e <- comp_com c r;
   mret (e, r).
 
-(* TODO: le is redundant ... fix up match_config *)
+(** We can "run" a computation the [CMD] monad by supplying it with empty lists
+of uids, labels, and blocks.  The result is easy to package up as ListCFG
+control-flow graph.  *)
+
 Definition compile (c:com) : ListCFG.t * lbl * lbl :=
   let '(_, _, bs, (le, lr)) := comp_prog c ([], [], []) in
     ((le, bs), le, lr).
