vminus/VminusOpSem.v
@@ -1,3 +1,5 @@
+(** VminusOpSem: Operational Semantics for Vminus *)
+
 Require Import Arith.
 Require Import List.
 Import ListNotations.
